feat: add simulation of the get function

CoqOfNoir/simulation/CoqOfNoir.v
@@ -1,5 +1,57 @@
 Require Import CoqOfNoir.CoqOfNoir.
 
+Module Panic.
+  Inductive t (A : Set) : Set :=
+  | Value : A -> t A
+  (** The [Panic] works with an existential type, so we can return any payload for errors. This is
+      useful for debugging. Then we cannot catch the error and compute with it as we do not know the
+      type anymore, but catching panic errors is not supposed to happen in Rust. *)
+  | Panic (payload : {Error : Set @ Error}) : t A.
+  Arguments Value {_}.
+  Arguments Panic {_}.
+
+  Definition return_ {A : Set} (value : A) : t A :=
+    Value value.
+
+  Definition panic {A Error : Set} (error : Error) : t A :=
+    Panic (existS _ error).
+
+  Definition bind {A B : Set} (value : t A) (f : A -> t B) : t B :=
+    match value with
+    | Value value => f value
+    | Panic error => Panic error
+    end.
+
+  Definition fold_left {A B : Set} (init : A) (l : list B) (f : A -> B -> t A) : t A :=
+    List.fold_left (fun acc x => bind acc (fun acc => f acc x)) l (return_ init).
+
+  Definition map {A B : Set} (l : list A) (f : A -> t B) : t (list B) :=
+    List.fold_right
+      (fun x acc => bind acc (fun acc => bind (f x) (fun x => return_ (x :: acc))))
+      (return_ []) l.
+End Panic.
+
+Module PanicNotations.
+  Notation "M!" := Panic.t.
+
+  Notation "return!" := Panic.return_.
+  Notation "panic!" := Panic.panic.
+
+  Notation "'let!' x ':=' X 'in' Y" :=
+    (Panic.bind X (fun x => Y))
+    (at level 200, x pattern, X at level 100, Y at level 200).
+
+  Notation "'do!' X 'in' Y" :=
+    (Panic.bind X (fun (_ : unit) => Y))
+    (at level 200, X at level 100, Y at level 200).
+
+  Notation "fold!" := Panic.fold_left.
+
+  Notation "map!" := Panic.map.
+End PanicNotations.
+
+Export PanicNotations.
+
 Module ToValue.
   Class Trait (Self : Set) : Set := {
     to_value : Self -> Value.t;
@@ -133,107 +185,154 @@ Module I64.
   }.
 End I64.
 
-Module Integer.
+Module SemiInteger.
   Class Trait (Self : Set) : Set := {
     to_Z : Self -> Z;
+  }.
+End SemiInteger.
+
+Global Instance Impl_SemiInteger_for_Field : SemiInteger.Trait Field.t := {
+  SemiInteger.to_Z (i : Field.t) :=
+    let 'Field.Make i := i in
+    i;
+}.
+
+Global Instance Impl_SemiInteger_for_U1 : SemiInteger.Trait U1.t := {
+  SemiInteger.to_Z (i : U1.t) :=
+    let 'U1.Make i := i in
+    i;
+}.
+
+Global Instance Impl_SemiInteger_for_U8 : SemiInteger.Trait U8.t := {
+  SemiInteger.to_Z (i : U8.t) :=
+    let 'U8.Make i := i in
+    i;
+}.
+
+Global Instance Impl_SemiInteger_for_U16 : SemiInteger.Trait U16.t := {
+  SemiInteger.to_Z (i : U16.t) :=
+    let 'U16.Make i := i in
+    i;
+}.
+
+Global Instance Impl_SemiInteger_for_U32 : SemiInteger.Trait U32.t := {
+  SemiInteger.to_Z (i : U32.t) :=
+    let 'U32.Make i := i in
+    i;
+}.
+
+Global Instance Impl_SemiInteger_for_U64 : SemiInteger.Trait U64.t := {
+  SemiInteger.to_Z (i : U64.t) :=
+    let 'U64.Make i := i in
+    i;
+}.
+
+Global Instance Impl_SemiInteger_for_I1 : SemiInteger.Trait I1.t := {
+  SemiInteger.to_Z (i : I1.t) :=
+    let 'I1.Make i := i in
+    i;
+}.
+
+Global Instance Impl_SemiInteger_for_I8 : SemiInteger.Trait I8.t := {
+  SemiInteger.to_Z (i : I8.t) :=
+    let 'I8.Make i := i in
+    i;
+}.
+
+Global Instance Impl_SemiInteger_for_I16 : SemiInteger.Trait I16.t := {
+  SemiInteger.to_Z (i : I16.t) :=
+    let 'I16.Make i := i in
+    i;
+}.
+
+Global Instance Impl_SemiInteger_for_I32 : SemiInteger.Trait I32.t := {
+  SemiInteger.to_Z (i : I32.t) :=
+    let 'I32.Make i := i in
+    i;
+}.
+
+Global Instance Impl_SemiInteger_for_I64 : SemiInteger.Trait I64.t := {
+  SemiInteger.to_Z (i : I64.t) :=
+    let 'I64.Make i := i in
+    i;
+}.
+
+Module Integer.
+  Class Trait (Self : Set) `{SemiInteger.Trait Self} : Set := {
     of_Z : Z -> Self;
   }.
 
+  Definition to_Z {Self : Set} `{Trait Self} (self : Self) : Z :=
+    SemiInteger.to_Z self.
+
+  Definition to_nat {Self : Set} `{Trait Self} (self : Self) : nat :=
+    Z.to_nat (to_Z self).
+
   Definition add {Self : Set} `{Trait Self} (self other : Self) : Self :=
-    of_Z (to_Z self + to_Z other).
+    of_Z (SemiInteger.to_Z self + SemiInteger.to_Z other).
 
   Definition sub {Self : Set} `{Trait Self} (self other : Self) : Self :=
-    of_Z (to_Z self - to_Z other).
+    of_Z (SemiInteger.to_Z self - SemiInteger.to_Z other).
 
   Definition mul {Self : Set} `{Trait Self} (self other : Self) : Self :=
-    of_Z (to_Z self * to_Z other).
+    of_Z (SemiInteger.to_Z self * SemiInteger.to_Z other).
 
   Definition div {Self : Set} `{Trait Self} (self other : Self) : Self :=
-    of_Z (to_Z self / to_Z other).
+    of_Z (SemiInteger.to_Z self / SemiInteger.to_Z other).
 
   Definition mod_ {Self : Set} `{Trait Self} (self other : Self) : Self :=
-    of_Z (to_Z self mod to_Z other).
+    of_Z (SemiInteger.to_Z self mod SemiInteger.to_Z other).
 
   Definition of_bool {Self : Set} `{Trait Self} (b : bool) : Self :=
     of_Z (if b then 1 else 0).
 End Integer.
 
 Global Instance Impl_Integer_for_U1 : Integer.Trait U1.t := {
-  Integer.to_Z (i : U1.t) :=
-    let 'U1.Make i := i in
-    i;
   Integer.of_Z (i : Z) :=
     U1.Make (i mod (2^1));
 }.
 
 Global Instance Impl_Integer_for_U8 : Integer.Trait U8.t := {
-  Integer.to_Z (i : U8.t) :=
-    let 'U8.Make i := i in
-    i;
   Integer.of_Z (i : Z) :=
     U8.Make (i mod (2^8));
 }.
 
 Global Instance Impl_Integer_for_U16 : Integer.Trait U16.t := {
-  Integer.to_Z (i : U16.t) :=
-    let 'U16.Make i := i in
-    i;
   Integer.of_Z (i : Z) :=
     U16.Make (i mod (2^16));
 }.
 
 Global Instance Impl_Integer_for_U32 : Integer.Trait U32.t := {
-  Integer.to_Z (i : U32.t) :=
-    let 'U32.Make i := i in
-    i;
   Integer.of_Z (i : Z) :=
     U32.Make (i mod (2^32));
 }.
 
 Global Instance Impl_Integer_for_U64 : Integer.Trait U64.t := {
-  Integer.to_Z (i : U64.t) :=
-    let 'U64.Make i := i in
-    i;
   Integer.of_Z (i : Z) :=
     U64.Make (i mod (2^64));
 }.
 
 Global Instance Impl_Integer_for_I1 : Integer.Trait I1.t := {
-  Integer.to_Z (i : I1.t) :=
-    let 'I1.Make i := i in
-    i;
   Integer.of_Z (i : Z) :=
     I1.Make (((i + 2^0) mod (2^1)) - 2^0);
 }.
 
 Global Instance Impl_Integer_for_I8 : Integer.Trait I8.t := {
-  Integer.to_Z (i : I8.t) :=
-    let 'I8.Make i := i in
-    i;
   Integer.of_Z (i : Z) :=
     I8.Make (((i + 2^7) mod (2^8)) - 2^7);
 }.
 
 Global Instance Impl_Integer_for_I16 : Integer.Trait I16.t := {
-  Integer.to_Z (i : I16.t) :=
-    let 'I16.Make i := i in
-    i;
   Integer.of_Z (i : Z) :=
     I16.Make (((i + 2^15) mod (2^16)) - 2^15);
 }.
 
 Global Instance Impl_Integer_for_I32 : Integer.Trait I32.t := {
-  Integer.to_Z (i : I32.t) :=
-    let 'I32.Make i := i in
-    i;
   Integer.of_Z (i : Z) :=
     I32.Make (((i + 2^31) mod (2^32)) - 2^31);
 }.
 
 Global Instance Impl_Integer_for_I64 : Integer.Trait I64.t := {
-  Integer.to_Z (i : I64.t) :=
-    let 'I64.Make i := i in
-    i;
   Integer.of_Z (i : Z) :=
     I64.Make (((i + 2^63) mod (2^64)) - 2^63);
 }.
@@ -253,7 +352,16 @@ Module Array.
   }.
 
   Definition repeat {A : Set} (size : U32.t) (value : A) : t A size :=
-    Make (List.repeat value (Z.to_nat (Integer.to_Z size))).
+    Make (List.repeat value (Z.to_nat (SemiInteger.to_Z size))).
+
+  Definition get {A Index: Set} `{SemiInteger.Trait Index} {size : U32.t}
+      (array : t A size) (index : Index) :
+      M! A :=
+    let 'Make array := array in
+    match List.nth_error array (Z.to_nat (SemiInteger.to_Z index)) with
+    | Some result => return! result
+    | None => panic! ("Array.get: index out of bounds", array, index)
+    end.
 End Array.
 
 Module Eq.
